lean/Shars/Verification/Simple/Iota.lean
@@ -7,13 +7,14 @@ import Aeneas.SimpLists.Init
 import Sha3.Facts
 import Init.Data.Vector.Lemmas
 import Init.Data.Nat.Basic
+import Shars.Verification.Simple.Constants
 import Shars.Verification.Simple.Utils
 import Shars.Verification.Simple.Auxiliary
 
 set_option maxHeartbeats 1000000
 
 open Aeneas hiding Std.Array
-open Std.alloc.vec 
+open Std.alloc.vec
 
 theorem simple.IOTA_RC_POINTS.spec
 : ∀ t < 255, IOTA_RC_POINTS.val[t]! = Spec.Keccak.ι.rc t
@@ -23,7 +24,7 @@ attribute [scalar_tac_simps] Nat.mod_mod Fin.ofNat'
 
 @[progress]
 theorem simple.iota_rc_point.spec(t: Std.Usize)
-: ∃ output, 
+: ∃ output,
   iota_rc_point t = .ok output ∧
   output = Spec.Keccak.ι.rc t.val
 := by
@@ -36,34 +37,7 @@ theorem simple.iota_rc_point.spec(t: Std.Usize)
     ←Spec.Keccak.ι.rc
   ]
 
-theorem Aeneas.Std.UScalar.one_ShiftLeft_spec {ty1}(ty0: UScalarTy)(y : UScalar ty1)
-  (hy : y.val < ty0.numBits)
-: ∃ z, (1#ty0.numBits#uscalar) <<< y = .ok z ∧
-  z.val = 2^y.val ∧
-  z.bv = 1#ty0.numBits <<< y.val
-  := by
-  simp only [HShiftLeft.hShiftLeft, shiftLeft_UScalar, shiftLeft, hy, reduceIte, UScalar.size]
-  simp only [BitVec.shiftLeft_eq, Result.ok.injEq, _root_.exists_eq_left', and_true, val]
-  simp only [HShiftLeft.hShiftLeft, shiftLeft_UScalar, shiftLeft, hy, reduceIte, UScalar.size]
-  simp only [bv_toNat, BitVec.shiftLeft_eq, BitVec.toNat_shiftLeft, BitVec.toNat_ofNat, Nat.shiftLeft_eq, Nat.mod_mul_mod, one_mul]
-  apply Nat.mod_eq_of_lt
-  apply Nat.pow_lt_pow_of_lt Nat.one_lt_two ‹y.val < ty0.numBits›
-
-/- theorem Aeneas.Std.Usize.one_ShiftLeft_spec {ty1}(ty0: UScalarTy)(y : UScalar ty1) (size : Nat) -/
-@[progress] theorem Aeneas.Std.Usize.one_ShiftLeft_spec (y : UScalar ty1) (hy : y.val < UScalarTy.Usize.numBits) 
-: ∃ (z : Usize),
-  1#usize <<< y = .ok z ∧
-  z.val = 2 ^ y.val ∧
-  z.bv = (1#usize).bv <<< y.val
-:= UScalar.one_ShiftLeft_spec _ _ hy
-
-/- @[scalar_tac 2 ^ n] -/ 
-/- theorem Nat.one_lt_two_pow''(n: Nat): 1 ≤ 2^n := @Nat.one_le_two_pow n -/
-attribute [scalar_tac_simps] Nat.one_le_two_pow
-
-@[simp, scalar_tac_simps] theorem simple.L.spec : L.val = 6 := by native_decide
-
-def simple.iota_rc_init_loop.ref(ir: Nat)(rc: BitVec (Spec.w 6))(j: Nat) := 
+def simple.iota_rc_init_loop.ref(ir: Nat)(rc: BitVec (Spec.w 6))(j: Nat) :=
   if j <= 6
   then
     let i := 7 * ir
@@ -76,21 +50,6 @@ def simple.iota_rc_init_loop.ref(ir: Nat)(rc: BitVec (Spec.w 6))(j: Nat) :=
     iota_rc_init_loop.ref ir rc1 j1
   else rc
 termination_by 7 - j
-
-@[scalar_tac Std.UScalarTy.Usize.numBits]
-theorem Std.UScalarTy.Usize_numBits_le: Std.UScalarTy.Usize.numBits ≥ 32 := by
-  rcases System.Platform.numBits_eq with h | h <;> simp [h]
-
-@[simp]
-theorem BitVec.ofBoolListLE_set(ls: List Bool)(i: Nat)(b: Bool)
-: {i_idx: i < ls.length}
-→ BitVec.ofBoolListLE (ls.set i b) = ((BitVec.ofBoolListLE ls).set ⟨i, i_idx⟩ b).cast (by simp)
-:= by
-  intro i_idx
-  ext j j_idx
-  simp at j_idx
-  simp [BitVec.getElem_set]
-  split <;> simp [*]
 
 theorem simple.iota_rc_init_loop.ref_spec(ir : Std.Usize) (input : Aeneas.Std.Array Bool 64#usize)(j: Std.Usize)
 : ir.val < 24
@@ -109,10 +68,10 @@ theorem simple.iota_rc_init_loop.ref_spec(ir : Std.Usize) (input : Aeneas.Std.Ar
     simp [i1_post, i_post] at b_post
     let* ⟨ i2, i2_post_1, i2_post_2 ⟩ ← Std.Usize.one_ShiftLeft_spec
     let* ⟨ i3, i3_post ⟩ ← Std.Usize.sub_spec
-    have i3_val: i3.val = i2.val - 1 := by 
+    have i3_val: i3.val = i2.val - 1 := by
       rw [i3_post, Nat.add_sub_cancel]
     simp [i2_post_1] at i3_val
-    have i3_idx: i3.val < input.length := by 
+    have i3_idx: i3.val < input.length := by
       simp [*]
       calc  2 ^ ↑j - 1
           _ < 2 ^ ↑j := Nat.pred_lt (Nat.ne_of_gt (Nat.two_pow_pos j.val))
@@ -137,11 +96,11 @@ termination_by 7 - j.val
 decreasing_by scalar_decr_tac
 
 theorem simple.iota_rc_init_loop.ref.foldWhile_spec(iᵣ: Nat)(input: BitVec (Spec.w 6))(j: Nat)
-: iota_rc_init_loop.ref iᵣ input j = SRRange.foldWhile 
-    (i    := j) 
-    (max  := 6 + 1) 
-    (step := 1) (hStep := Nat.one_pos) 
-    (init := input) 
+: iota_rc_init_loop.ref iᵣ input j = SRRange.foldWhile
+    (i    := j)
+    (max  := 6 + 1)
+    (step := 1) (hStep := Nat.one_pos)
+    (init := input)
     (f    := fun input j => input.set (↑(1 <<< j - 1)) (Spec.Keccak.ι.rc (j + 7 * iᵣ)))
 := by
   rw [ref, SRRange.foldWhile]
@@ -157,23 +116,14 @@ def Spec.Keccak.ι.RC.loop (iᵣ: Nat)(init: BitVec (w 6))(start: Nat): BitVec (
     have j_valid_idx := calc  2 ^ ↑j - 1
         _ < 2 ^ ↑j := Nat.pred_lt (Nat.ne_of_gt (Nat.two_pow_pos j.val))
         _ ≤ 2 ^ 6 := Nat.pow_le_pow_right Nat.two_pos <| Fin.is_le j
-    RC := RC.set ⟨2^j.val - 1, j_valid_idx⟩ (ι.rc (↑j + 7*iᵣ)) 
+    RC := RC.set ⟨2^j.val - 1, j_valid_idx⟩ (ι.rc (↑j + 7*iᵣ))
   return RC
 
-def BitVec.set!{n: Nat}(i: Nat)(b: Bool)(bv: BitVec n): BitVec n := 
-  if _: i < n then
-    bv.set ⟨i, ‹i < n›⟩ b
-  else bv
-
-theorem BitVec.set!_eq_set{n: Nat}(i: Nat)(b: Bool)(bv: BitVec n)⦃i_idx: i < n⦄
-: bv.set! i b = bv.set ⟨i, i_idx⟩ b
-:= by simp only [set!, reduceDIte, i_idx]
-
-def Spec.Keccak.ι.RC.loop.spec(iᵣ: Nat)
+theorem Spec.Keccak.ι.RC.loop_refinement(iᵣ: Nat)
 : RC.loop iᵣ (0#(w 6)) 0 = RC iᵣ
 := by simp [loop, RC]; congr
 
-def Spec.Keccak.ι.RC.loop.foldl_spec(iᵣ: Nat)(init: BitVec (w 6))(start: Nat)
+theorem Spec.Keccak.ι.RC.loop.foldl_spec(iᵣ: Nat)(init: BitVec (w 6))(start: Nat)
 : RC.loop iᵣ init start =
     List.foldl (fun RC j => RC.set! (2^j - 1) (ι.rc (j + 7*iᵣ))) init (List.range (6 + 1) |>.drop start)
 := by
@@ -186,7 +136,7 @@ def Spec.Keccak.ι.RC.loop.foldl_spec(iᵣ: Nat)(init: BitVec (w 6))(start: Nat)
   ext RC j : 2
   rw [BitVec.set!_eq_set]
 
-theorem Aeneas.SRRange.foldWhile_eq_foldWhile'{α : Type u} 
+theorem Aeneas.SRRange.foldWhile_eq_foldWhile'{α : Type u}
 (i max step : Nat) (hStep : 0 < step) (f : α → Nat → α) (init : α)(start: Nat)
 : (cond: start ≤ i ∧ (i - start) % step = 0)
 → foldWhile max step hStep f i init = SRRange.foldWhile' {
@@ -209,11 +159,11 @@ theorem Aeneas.SRRange.foldWhile_eq_foldWhile'{α : Type u}
 termination_by max - i
 
 def simple.iota_rc_init_loop.foldWhile.spec(iᵣ: Nat)(init: BitVec (Spec.w 6))(start: Nat)
-: SRRange.foldWhile 
-    (i    := start) 
-    (max  := 6 + 1) 
-    (step := 1) (hStep := Nat.one_pos) 
-    (init := init) 
+: SRRange.foldWhile
+    (i    := start)
+    (max  := 6 + 1)
+    (step := 1) (hStep := Nat.one_pos)
+    (init := init)
     (f    := fun input j => BitVec.set (1 <<< j - 1).cast (Spec.Keccak.ι.rc (j + 7 * iᵣ)) input)
 = Spec.Keccak.ι.RC.loop iᵣ init start
 := by
@@ -253,22 +203,17 @@ theorem simple.iota_rc_init_loop.spec(ir : Std.Usize) (input : Aeneas.Std.Array 
     simple.iota_rc_init_loop.foldWhile.spec,
   ]
 
-theorem repeat_false_toBitVec_eq_zero(size: Std.Usize)
-: (Std.Array.repeat size false).val.toBitVec = (0#(size.val)).cast (by simp)
-:= by ext i; simp only [Std.Array.repeat, BitVec.getElem_cast,
-  BitVec.getElem_ofBoolListLE, List.getElem_replicate, BitVec.getElem_zero]
-
 @[progress]
 theorem simple.iota_rc_init.spec(ir: Std.Usize)
 : ir.val < 24
 → ∃ output,
   simple.iota_rc_init ir (Std.Array.repeat 64#usize false) = .ok output ∧
   output.val.toBitVec.cast (by simp [Spec.w]) = (Spec.Keccak.ι.RC ir.val : BitVec (Spec.w 6))
-:= by 
+:= by
   intro ir_lt
   simp [iota_rc_init]
   let* ⟨output , output_post⟩ ← iota_rc_init_loop.spec
-  rw [output_post, ←Spec.Keccak.ι.RC.loop.spec]
+  rw [output_post, ←Spec.Keccak.ι.RC.loop_refinement]
   congr
   ext i i_idx
   simp only [Std.Array.repeat, BitVec.getElem_cast,
@@ -276,11 +221,11 @@ theorem simple.iota_rc_init.spec(ir: Std.Usize)
 
 
 @[progress]
-theorem simple.iota_a_loop.spec(res : StateArray) (a : StateArray) (rc : Aeneas.Std.Array Bool 64#usize)(z: Std.Usize) 
+theorem simple.iota_a_loop.spec(res : StateArray) (a : StateArray) (rc : Aeneas.Std.Array Bool 64#usize)(z: Std.Usize)
 : ∃ output,
   simple.iota_a_loop res a rc z = .ok output ∧
   ∀ (x y: Fin 5)(z': Fin (Spec.w 6)),
-  output.toSpec.get x y z' = 
+  output.toSpec.get x y z' =
     if x = 0 ∧ y = 0 ∧ z.val ≤ z'.val then
       a.toSpec.get 0 0 z' ^^ rc.val.toBitVec[z'.val]!
     else
@@ -307,7 +252,7 @@ theorem simple.iota_a_loop.spec(res : StateArray) (a : StateArray) (rc : Aeneas.
       simp only [Fin.isValue, zz', Fin.cast_val_eq_self, and_true]--, ite_eq_left_iff, not_and]
       simp_ifs
     · rw [Spec.Keccak.StateArray.get_set]
-      have: ¬ (x = 0 ∧ y = 0 ∧ z' = z.val.cast) := by 
+      have: ¬ (x = 0 ∧ y = 0 ∧ z' = z.val.cast) := by
         -- TODO: Could we modify `scalar_tac` so that it handles this case?
         -- The issue is with `Fin` inequalities being hiden behind `And`, `Or` or `Not`.
         -- It would be nice to have `scalar_tac` transform these using the lemmas
@@ -315,7 +260,7 @@ theorem simple.iota_a_loop.spec(res : StateArray) (a : StateArray) (rc : Aeneas.
         --  · Fin.val_inj
         -- I was thinking of using a `simproc`, but I don't think these work with
         -- implications, since they're supposed to do rewritings.
-        -- Perhaps I could have it 
+        -- Perhaps I could have it
         rename_i h1 h2
         simp [not_and_or, -not_and] at h1 h2 ⊢
         rcases h1 with (h1 | h1 | h1) <;> try simp [h1]
