lean/Shars/Verification/Simple.lean
@@ -1,0 +1,1 @@
+import Shars.Verification.Simple.Sponge
